theories/CTree/Logic/AG.v
@@ -33,427 +33,63 @@ Section BasicLemmas.
 
   Lemma ag_now: forall e (k: encode e -> ctree E X)
                   (v : encode e) w φ,
-      (φ w /\ not_done w /\
-         forall v, <( {k v}, {Obs e v} |= AG now φ )>) <->
-        <( {Vis e k}, w |= AG now φ )>.
+      (<( {Vis e k}, w |= φ )> /\ forall v, <( {k v}, {Obs e v} |= AG φ )>) <->
+         <( {Vis e k}, w |= AG φ )>.
   Proof with eauto with ctl.
     split; intros.
-    - destruct H as (Hφ & Hd & H).
-      next; split.
-      + inv Hd.
-        * apply ctl_now...
-        * apply ctl_now...          
-      + apply ax_vis... 
-    - next in H; cdestruct H.  
-      destruct H0 as (Hs & Ht').
-      apply ctl_now in H as (? & ?).
-      split; [|split]...
+    - destruct H as (Hφ & H).      
+      csplit...
+      + apply ctll_not_done in Hφ.
+        apply can_step_vis...
+      + intros t' w' TR.
+        apply ktrans_vis in TR as (v' & -> & <- & ?)...
+    - cdestruct H.
+      split...
       intro v'.
-      rewrite unfold_entailsF.
-      apply Ht', ktrans_vis...
+      apply H, ktrans_vis...
   Qed.
   
   Lemma ag_br: forall n (k: fin' n -> ctree E X) w φ,
-      (not_done w /\
-         forall (i: fin' n), <( {k i}, w |= AG now φ )>) <->
-        <( {Br n k}, w |= AG now φ )>.
-  Proof with auto with ctl.
+      (<( {Br n k}, w |= φ )> /\ forall (i: fin' n), <( {k i}, w |= AG φ )>) <->
+        <( {Br n k}, w |= AG φ )>.
+  Proof with eauto with ctl.
     split; intros.
-    - destruct H as (Hd & H).
-      next; split.
-      + specialize (H Fin.F1).
-        next in H.
-        destruct H.
-        now cbn in *.
-      + apply ax_br... 
-    - next in H; cdestruct H.       
-      destruct H0 as (Hs & Ht').
-      apply ctl_now in H as (? & ?).
+    - destruct H as (Hφ & H).
+      csplit...
+      + apply ctll_not_done in Hφ.
+        apply can_step_br...
+      + intros t' w' TR.
+        apply ktrans_br in TR as (i' & -> & -> & Hd).
+        apply H.
+    - cdestruct H.
       split...
       intro i.
-      rewrite unfold_entailsF.
-      apply Ht', ktrans_br.
-      exists i...
+      apply H, ktrans_br...
   Qed.
 
   Lemma ag_stuck: forall w φ,
-      <( {stuck: ctree E X}, w |= AG φ )> -> False.
+      ~ <( {stuck: ctree E X}, w |= AG φ )>.
   Proof.
-    intros.
+    intros * H.
     cdestruct H; subst. 
-    destruct H as (? & (Hs & ?)).
     now apply can_step_stuck in Hs.
   Qed.
 
   Lemma ag_ret: forall (x: X) w φ,      
-      <( {Ret x}, w |= AG φ )> -> False.
+      ~ <( {Ret x}, w |= AG φ )>.
   Proof.
-    intros. 
+    intros * H. 
     cdestruct H.
-    destruct H as (? & ((t' & w' & TR) & ?)). 
-    specialize (H0 _ _ TR).
-    cbn in TR.
-    dependent destruction TR; observe_equ x;
-      rewrite <- Eqt, H0 in H1; eapply ag_stuck;
-      rewrite unfold_entailsF; apply H1.
+    destruct Hs as (t' & w' & TR).    
+    specialize (H _ _ TR).
+    apply ctll_not_done in Hp.
+    inv Hp.
+    + apply ktrans_done in TR as (-> & ?).
+      rewrite H0 in H.
+      now apply ag_stuck in H.
+    + apply ktrans_finish in TR as (-> & ?).
+      rewrite H0 in H.
+      now apply ag_stuck in H.
   Qed.
 
-  Lemma ag_guard: forall w φ (t: ctree E X),
-      <( {Guard t}, w |= AG φ )> <-> <( t, w |= AG φ )>.
-  Proof.
-    intros.
-    now rewrite sb_guard.
-  Qed.
 End BasicLemmas.
-
-Section BindLemmas.
-  Context {E: Type} {HE: Encode E}.
-
-  (* [t] will loop forever. *)
-  Lemma ag_bind_l{X Y}: forall (t: ctree E X) w (k: X -> ctree E Y) φ,
-      <( t, w |= AG now φ )> ->
-      <( {x <- t ;; k x} , w |= AG now φ )>.
-  Proof.    
-    intros.
-    generalize dependent t.
-    revert k w.
-    coinduction R CIH; intros; constructor; step in H; destruct H; intuition.
-    destruct H0 as ((t' & w' & TR) & ?).
-    split.
-    - apply can_step_bind.
-      left.      
-      exists t', w'; intuition.
-      specialize (H0 t' w' TR).
-      step in H0; ddestruction H0; intuition.
-      destruct H1.
-      now apply can_step_not_done with t'.
-    - intros k_ w_ TR_.
-      apply ktrans_bind_inv in TR_ as
-          [(t_ & TRt & Hd & ->) |
-            (x & wx & TR' & Hr & TRk)].
-      + apply CIH.
-        rewrite unfold_entailsF.
-        now apply H0.
-      + specialize (H0 _ _ TR').
-        step in H0; ddestruction H0; intuition.
-        destruct H1.
-        now apply can_step_stuck in H1.
-  Qed.
-
-  Typeclasses Transparent sbisim.
-  Typeclasses Transparent equ.
-  Lemma ag_iter_l{X I}: forall (k: I -> ctree E (I + X)) i w (x: I) φ,
-      <( {k i}, w |= AG now φ )> ->
-      <( {iter k i}, w |= AG now φ )>.
-  Proof.
-    intros.
-    rewrite sb_unfold_iter.
-    now apply ag_bind_l.
-  Qed.
-
-  Notation MP X := (rel (ctree E X) (World E)).
-  Program Definition ag_bind_now_clos{X Y} φ Post : mon (MP Y) :=
-    {| body R t w :=
-        bind_ctx1
-          (fun (t: ctree E X) => <( t, w |= now φ AU (AX done Post) )>)
-          (fun (k: X -> ctree E Y) =>
-             forall (x: X) (w: World E), Post x w -> R (k x) w)
-          t
-    |}.
-  Next Obligation.
-    revert H0.
-    apply leq_bind_ctx1; intros.
-    apply in_bind_ctx1; eauto.
-  Qed.
-
-  Lemma ag_bind_now_ag{X Y} φ Post:
-      ag_bind_now_clos (X:=X) (Y:=Y) φ Post <= cagt <( |- now φ )>.
-  Proof.    
-    apply Coinduction.
-    intros R t w; cbn.
-    apply (leq_bind_ctx1 _ _
-             (fun t => cagF (entailsF <( now φ )>)
-                      (cagT (entailsF <( now φ )>)
-                         (ag_bind_now_clos φ Post) R) t w)). 
-    intros x Hx k Hk.
-    cinduction Hx.
-    - (* AX done R *)
-      apply ax_done in H as (Hw & x & Heq & HPost).
-      specialize (Hk _ _ HPost); remember (k x) as K;
-        destruct Hk; subst; split.      
-      + rewrite Heq, bind_ret_l; try (exact (equ eq)); auto.
-      + split.
-        * rewrite Heq, bind_ret_l.
-          now destruct H0.
-        * intros t' w' TR.
-          apply (id_T (cagF (entailsF <( now φ )>))); cbn.
-          destruct H0.
-          apply H1.
-          eapply ktrans_sbisim_ret with (t:=t0); auto.
-    - (* vis φ *)
-      destruct H0, H1; clear H0.
-      destruct H1 as (t' & w' & TR).
-      split; [auto | split].
-      + apply can_step_bind_l with t' w'; auto.
-        destruct (H3 _ _ TR); try contradiction.
-        destruct H1.
-        now apply ctl_now in H0.
-      + intros k_ w_ TRk.
-        apply ktrans_bind_inv in TRk as
-            [(t0' & TR0 & Hd_ & Heq) | (x & w0 & TRt0 & Hd & TRk)].
-        * (* [t0] steps and is not [Ret] *)
-          apply (fT_T (mequ_clos_cag (KS:=KripkeSetoidEqu))).
-          cbn; eapply mequ_clos_ctor with (t1:=x <- t0';; k x) (w1:=w_); auto.
-          clear Heq k_.            
-          eapply (fTf_Tf (cagF <( |- now φ )>)). 
-          apply in_bind_ctx1.
-          -- rewrite unfold_entailsF; auto.             
-          -- intros.
-             apply (b_T (cagF <( |- now φ )>)); cbn; auto.
-        * (* [t0] steps and is [Ret], contradiction *)
-          ddestruction Hd; subst;
-            specialize (H3 _ _ TRt0); ddestruction H3;
-            try contradiction;
-            destruct H1, H0;
-            rewrite can_step_bind in H1;
-            destruct H1 as [(? & ? & TRinv & ?) | (? & ? & TRinv & ?)];
-            now apply ktrans_stuck in TRinv.
-  Qed.
-
-  (* [t] satisfies [φ] until it terminates with post-condition [R],
-     then forall x w, R x w -> k x, w satisfies [φ] forever. *)
-  Lemma ag_bind_r{X Y}: forall (t: ctree E X)
-                          w (k: X -> ctree E Y) φ R,
-      <( t, w |= now φ AU AX done R )> ->
-      (forall (x: X) (w: World E), R x w -> <( {k x}, w |= AG now φ )>) ->
-      <( {x <- t ;; k x} , w |= AG now φ )>.
-  Proof.
-    intros.
-    rewrite unfold_entailsF.
-    apply (ft_t (ag_bind_now_ag φ R)).
-    cbn.
-    apply in_bind_ctx1; auto.
-  Qed.
-
-  Lemma ag_iter{X I}: forall (k: I -> ctree E (I + X)) w (x: I) φ R,
-      R x ->          (* Iterator invariant: [x] in [R] *)
-      φ w ->          (* Worlds invariant: [φ w] *)
-      not_done w ->
-      (forall (i: I) (w: World E),
-          R i ->
-          not_done w ->
-          φ w ->
-          <( {k i}, w |= AX (now φ AU AX done
-                 {fun (lr: I+X) (w: World E) =>
-                    exists i' : I, lr = inl i' /\ φ w /\ not_done w /\ R i'}))>) ->
-      <( {iter k x}, w |= AG now φ )>.
-  Proof with auto with ctl.
-    (* Coinduction steps *)
-    intros.
-    generalize dependent x.
-    generalize dependent w.    
-    coinduction RR CIH; intros.
-    split.
-    - apply ctl_now; auto.
-    - split. 
-      + (* can_step (iter k x) w *)
-        specialize (H2 _ _ H H1 H0) as HAX.
-        cdestruct HAX.
-        destruct Hs as (k' & w' & TR).
-        rewrite sb_unfold_iter.
-        specialize (HAX _ _ TR); cdestruct HAX.
-        * apply ax_done in H3 as (Hd & y & Hy & i & -> & ? & _ & ?).
-          apply can_step_bind_l with k' w0... 
-        * destruct H4.
-          apply can_step_bind_l with k' w0...
-          apply ctl_now in H3 as (? & ?)...
-      + (* coinductive step *)
-        intros t' w' TR.
-        rewrite unfold_iter in TR.
-        apply ktrans_bind_inv in TR as
-            [(t0' & TR0 & Hd_ & Heq) | (x' & w0 & TRt0 & Hd & TRk)].
-        * (* [k x] steps *)
-          rewrite Heq; clear Heq t'.
-          apply (ft_t (ag_bind_now_ag φ
-             (fun (lr: I+X) (w0: World E) =>
-                exists i' : I, lr = inl i' /\ φ w0 /\ not_done w0 /\ R i'))); cbn.
-          apply in_bind_ctx1.
-          -- specialize (H2 _ _ H H1 H0) as HAX.
-             cdestruct HAX...
-          -- intros [l | r] w_ (i & Hinv & Hφ & Hd & HR); inv Hinv.
-             rewrite sb_guard.
-             apply CIH...
-        * (* [k x] returns *)        
-          specialize (H2 _ _ H H1 H0) as HAX.        
-          cdestruct HAX.
-          specialize (HAX _ _ TRt0).
-          apply au_stuck in HAX.
-          cdestruct HAX.
-          now apply can_step_stuck in Hs0.
-  Qed.
-  
-End BindLemmas.
-
-(*| Combinators for [interp_state] |*)
-Section CtlAgState.
-  Context {E F S: Type} {HE: Encode E} {HF: Encode F}
-    (h: E ~> stateT S (ctree F)).
-
-  Theorem ag_state_bind_l{X Y}: forall s w (t: ctree E Y) (k: Y -> ctree E X) φ,
-      <( {interp_state h t s}, w |= AG now φ )> ->
-      <( {interp_state h (x <- t ;; k x) s}, w |= AG now φ )>.
-  Proof.
-    intros.
-    rewrite interp_state_bind.
-    now apply ag_bind_l.
-  Qed.
-
-  Theorem ag_state_bind_r{X Y}: forall s (t: ctree E Y) (k: Y -> ctree E X) w φ
-                                  (R: Y -> S -> World F -> Prop),
-      <( {interp_state h t s}, w |= now φ AU (AX done {fun '(x, s) w => R x s w}) )> ->
-      (forall (y: Y) (s: S) (w: World F),
-          R y s w ->
-          <( {interp_state h (k y) s}, w |= AG now φ )>) ->
-      <( {interp_state h (x <- t ;; k x) s} , w |= AG now φ )>.
-  Proof.
-    intros.
-    rewrite interp_state_bind.
-    apply ag_bind_r with (R:=fun '(x, s) w => R x s w); auto.
-    intros [y s'] w' Hr; auto.
-  Qed.
-
-  Theorem ag_state_iter{X I}: forall s (k: I -> ctree E (I + X)) w (x: I) φ R,
-      R x s ->        (* Iterator invariant: [x] in [R] *)
-      φ w ->          (* Worlds invariant: [φ w] *)
-      not_done w ->
-      (forall (x: I) (s: S) (w: World F),
-          R x s ->
-          φ w ->
-          not_done w ->
-          <( {interp_state h (k x) s}, w |= AX (now φ AU AX done
-             {fun (lr: (I+X) * S) (w: World F) =>
-                exists (i' : I) (s': S), lr = (inl i', s') /\ φ w /\
-                                      not_done w /\ R i' s'}))>) ->
-      <( {interp_state h (iter k x) s}, w |= AG now φ )>.
-  Proof with auto with ctl.
-    intros.
-    rewrite interp_state_unfold_iter.
-    generalize dependent x.
-    generalize dependent s.
-    generalize dependent w.
-    coinduction RR CIH; intros.
-    split; [apply ctl_now; now constructor|split].
-    - (* can_step *)
-      specialize (H2 _ _ _ H H0 H1).
-      cdestruct H2.
-      destruct Hs as (t' & w' & TR).
-      specialize (H2 _ _ TR).
-      apply can_step_bind_l with t' w'; auto.
-      cdestruct H2.
-      + now apply ax_done in H2 as (? & ?).
-      + now apply ctl_now in H2 as (? & ?). 
-    - intros t' w' TR.
-      apply ktrans_bind_inv in TR as
-          [(t0' & TR0 & Hd_ & Heq) | (x' & w0 & TRt0 & Hd & TRk)].
-      + (* [k x] steps *)
-        rewrite Heq; clear Heq t'.
-        apply (ft_t (ag_bind_now_ag φ
-                       (fun (lr: (I+X) * S) (w: World F) =>
-                          exists (i': I) (s': S), lr = (inl i', s') /\
-                                               φ w /\ not_done w /\ R i' s'))); cbn.
-        apply in_bind_ctx1.
-        * specialize (H2 _ _ _ H H0 H1) as HAX.
-          cdestruct HAX.
-          specialize (HAX _ _ TR0).
-          apply HAX.
-        * intros (lr' & s_) w_ (i & s' & Hinv & Hφ & Hd' & HR'); inv Hinv.
-          rewrite sb_guard.
-          setoid_rewrite interp_state_unfold_iter.
-          apply CIH...
-      + (* [k x] returns *)        
-        specialize (H2 _ _ _ H H0 H1) as HAX.        
-        cdestruct HAX.
-        specialize (HAX _ _ TRt0).
-        apply au_stuck in HAX.
-        cdestruct HAX.
-        now apply can_step_stuck in Hs0.
-  Qed.        
-End CtlAgState.
-
-Section CtlAgW.
-  Context {E Σ W: Type} {HE: Encode E} (h:E ~> stateT Σ (ctreeW W)). 
-
-  Theorem ag_iterW{X I}: forall (i: I) (σ: Σ) (w: W) (k: I -> ctree E (I + X)) φ R,
-      R i σ ->       (* Iterator & state invariant [R] *)
-      φ w ->         (* Goal Invariant [φ] *)
-      (forall (i: I) (σ: Σ) (w: W),
-          R i σ ->
-          φ w ->
-          <( {interp_state h (k i) σ}, {Obs (Log w) tt} |=
-              AX (visW φ AU AX
-                    (finishW {fun (lr: I + X) (σ: Σ) (w: W) =>
-                                exists (i: I), lr = inl i /\ R i σ /\ φ w})))>) ->
-      <( {interp_state h (iter k i) σ}, {Obs (Log w) tt} |= AG visW φ )>.
-  Proof with eauto with ctl.
-    setoid_rewrite ctl_vis_now.
-    setoid_rewrite ctl_finish_done.
-    intros.
-    rewrite interp_state_unfold_iter.
-    generalize dependent σ.
-    generalize dependent i.
-    generalize dependent w.    
-    coinduction RR CIH; intros.
-    split; [apply ctl_now; eauto with ctl |split].
-    - (* can_step *)
-      specialize (H1 _ _ _ H H0).
-      cdestruct H1.
-      destruct Hs as (t' & w' & TR).
-      specialize (H1 _ _ TR).
-      apply can_step_bind_l with t' w'...
-      cdestruct H1.
-      + apply ax_done in H1 as (? & ?)...
-      + apply ctl_now in H1; destruct H1...
-    - intros t' w' TR.
-      apply ktrans_bind_inv in TR as
-          [(t0' & TR0 & Hd_ & Heq) | (x' & w0 & TRt0 & Hd & TRk)].
-      + (* [k x] steps *)
-        rewrite Heq; clear Heq t'.
-        apply (ft_t (ag_bind_now_ag
-                       (fun w => (exists (e : writerE W) (v : encode e),
-                                  w = Obs e v /\
-                                    (let 'Log v0 as x := e return (encode x -> Prop) in
-                                     fun 'tt => φ v0) v))
-                       (fun (x : (I + X) * Σ) (w : World (writerE W)) =>
-                        exists (e : writerE W) (v : encode e),
-                          w = Obs e v /\
-                          (let
-                           '(x0, s) := x in
-                            fun pat0 : writerE _ =>
-                            let
-                              'Log w0 as u := pat0 return (encode u -> Prop) in
-                            fun 'tt => exists i' : I, x0 = inl i' /\ R i' s /\ φ w0)
-                            e v))); cbn.
-        apply in_bind_ctx1.
-        * specialize (H1 _ _ _ H H0) as HAX.
-          cdestruct HAX.
-          specialize (HAX _ _ TR0).
-          apply HAX.
-        * intros (lr' & s_) w_ ([σ'] & [] & ? & ? & i' & ? & ?); subst.
-          unfold Classes.iter, MonadIter_ctree.          
-          apply (ft_t (mequ_clos_cag (KS:=KripkeSetoidSBisim))); cbn.
-          econstructor.
-          rewrite sb_guard.
-          rewrite interp_state_unfold_iter.
-          reflexivity.
-          reflexivity.
-          apply CIH...
-      + (* [k x] returns *)        
-        specialize (H1 _ _ _ H H0) as HAX.        
-        cdestruct HAX.
-        specialize (HAX _ _ TRt0).
-        apply au_stuck in HAX.
-        cdestruct HAX.
-        now apply can_step_stuck in Hs0.
-  Qed.        
-
-End CtlAgW.
